---
title: "Derivatives of 1/x and square root of x"
date: 2022-08-29T17:10:40-05:00
author: "Hongtao Hao"
slug: two-derivatives
draft: false
toc: true
tags: ML
---

## 1. `$y = \frac{1}{x}$`

The derivative of `$y = \frac{1}{x}$` can be computed in the following way.

First, I highly recommend you to watch [this clip](https://youtu.be/S0_qX4VJhMQ?list=PLZHQObOWTQDMsr9K-rj53DwVRMYO3t5Yr&t=605), where 3blue1brown visualizes this function. 

{{<figure src="/media/enblog/ml/1_x.png">}}

The key part of the proof is that Since A and B are both on the curve of `$y = \frac{1}{x}$`, the x coordinate times the y coordinate is 1. That is to say: `$A_x \cdot A_y = 1$` and `$B_x \cdot B_y = 1$`. If you know this, then you'll know that the areas of the two shaded areas are equal. Therefore,

$$dx \cdot (\frac{1}{x} - df) = x \cdot df$$

We have:

$$x\cdot df = \frac{dx}{x} - dx\cdot df$$

So:

$$x = \frac{dx}{x \cdot df} - dx$$

Because `$dx$` is extremely small, we can safely ignore it, and therefore, we have:

$$x = \frac{dx}{x \cdot df}$$

Multiply the above equation by $x$ and we have:

$$x^2 = \frac{dx}{df}$$

So we have:

$$\frac{df}{dx} = \frac{1}{x^2} = x^{-2}$$

Because `$df$` is negative, the derivative should be negative as well, so:

$$\frac{df}{dx} = - \frac{1}{x^2} = - x^{-2}$$

This method is inspired by [F J](https://i.imgur.com/R1cxqsm.png).

## 2. `$y = \sqrt{x}$`

It can be proven in two ways. 

### Intuitive way

First, let's use the way suggested by 3blue1brown.

{{<figure src="/media/enblog/ml/sqrt_x.png" caption="Source: Chapter 3 of Essence of calculus by 3blue1brown">}}

I'll write `$d\sqrt{x}$` as `$dy$`.

We have 

$$dx = 2\sqrt{x}\cdot dy + (dy)^2$$

Divide the equation by `$dy$` and we have:

$$2\sqrt{x} + dy = \frac{dx}{dy}$$

Therefore,

$$\frac{dy}{dx} = \frac{1}{2\sqrt{x} + dy}$$

Because `$dy$` is approaching zero, we can safely ignore it and we have

$$\frac{dy}{dx} = \frac{1}{2\sqrt{x}} = \frac{1}{2}x^{-\frac{1}{2}}$$

### Chain rule

Let's say we have `$f(x) = \sqrt{x}$`, `$g(x) = x^2$`, and `$h(x) = g(f(x)) = (\sqrt{x})^2 = x$`.

We have:

\begin{align}
h^\prime(x) & = 1 = g^\prime(f(x)) \cdot f^\prime(x)\\\\
& = 2\cdot f(x) \cdot f^\prime(x) \\\\
& = 2\sqrt{x} \cdot f^\prime(x) \\\\
\end{align}

So we have

$$f^\prime(x) = \frac{1}{2\sqrt{x}}$$

The method by chain rule is inspired by Yifan Wei. 